Add safety of systemF_rec

theories/language.v
@@ -1,6 +1,7 @@
 From Coq.Unicode Require Import Utf8.
 From Coq.Lists Require Import List.
 From Coq.Relations Require Import Relations.
+From Coq.micromega Require Import Lia.
 
 Class valid_language {expr : Type}
     (is_val : expr → Prop)
@@ -30,6 +31,11 @@ Inductive step {expr is_val is_ectx head_step} `{@valid_language expr is_val is_
 Definition steps {expr is_val is_ectx head_step} `{@valid_language expr is_val is_ectx head_step} :=
   clos_refl_trans _ step.
 
+Inductive nsteps {expr is_val is_ectx head_step} `{@valid_language expr is_val is_ectx head_step} :
+  nat → expr → expr → Prop :=
+| NSO e : nsteps 0 e e
+| NSS n e1 e2 e3 : step e1 e2 → nsteps n e2 e3 → nsteps (S n) e1 e3.
+
 Definition det_head_step
   {expr is_val is_ectx head_step} `{@valid_language expr is_val is_ectx head_step} e e' :=
   head_step e e' ∧ ∀ e'', head_step e e'' → e'' = e'.
@@ -40,6 +46,23 @@ Definition det_step
 
 Section language.
   Context {expr is_val is_ectx head_step} `{@valid_language expr is_val is_ectx head_step}.
+
+  Lemma nsteps_refl e : nsteps 0 e e.
+  Proof. constructor; fail. Qed.
+
+  Lemma step_nsteps e e' : step e e' → nsteps 1 e e'.
+  Proof. econstructor; [eassumption|econstructor]. Qed.
+
+  Lemma nsteps_trans n n' e e' e'' : nsteps n e e' → nsteps n' e' e'' → nsteps (n + n') e e''.
+  Proof.
+    induction 1; [trivial; fail|].
+    simpl.
+    econstructor; [eassumption|auto].
+  Qed.
+
+  Lemma nsteps_take_step n e e' e'' :
+    step e e' → nsteps n e' e'' → nsteps (S n) e e''.
+  Proof. intros ? ?; eapply (nsteps_trans 1); [apply step_nsteps|]; eauto. Qed.
 
   Lemma steps_ind (P : expr → expr → Prop) :
     (∀ e, P e e) →
@@ -61,6 +84,18 @@ Section language.
   Lemma steps_trans e e' e'' : steps e e' → steps e' e'' → steps e e''.
   Proof. econstructor; eauto; fail. Qed.
 
+  Lemma steps_nsteps e e' : steps e e' → ∃ n, nsteps n e e'.
+  Proof.
+    induction 1 as [| |? ? ? ? [n Hn] ? [k Hk]];
+      [eexists; eapply step_nsteps; assumption|exists 0; apply nsteps_refl|].
+    eexists (_ + _); eapply nsteps_trans; eauto.
+  Qed.
+
+  Lemma nsteps_steps n e e' : nsteps n e e' → steps e e'.
+  Proof.
+    induction 1; [econstructor; fail|eapply steps_trans; [apply step_steps; eassumption|trivial]].
+  Qed.
+
   Lemma val_no_step e : is_val e → ∀ e', ¬ step e e'.
   Proof.
     intros He e' Hstp.
@@ -71,10 +106,14 @@ Section language.
 
   Lemma val_steps_eq e e' : is_val e → steps e e' → e = e'.
   Proof.
-    induction 2 as [| |???? IH1 ? IH2]; subst; [|trivial; fail|].
-    - exfalso; eapply val_no_step; eauto.
-    - assert (x = y) by (apply IH1; trivial); subst.
-      apply IH2; trivial.
+    intros Hiv Hstps; revert Hiv.
+    pattern e; pattern e'.
+    match goal with
+    | |- (λ e', (λ e, ?P) _) _ => simpl; apply (steps_ind (λ e e', P))
+    end; [| |assumption]; clear e' e Hstps.
+    - trivial.
+    - intros ???????.
+      exfalso; eapply val_no_step; eauto.
   Qed.
 
   Lemma head_step_step e e' : head_step e e' → step e e'.
@@ -186,33 +225,35 @@ Section language.
     eapply Safe_det_step_back; [apply det_head_step_det_step|]; eassumption.
   Qed.
 
+  Lemma steps_under_ectx K e e' :
+    is_ectx K → steps (K e) e' →
+    (∃ e'', e' = K e'' ∧ steps e e'') ∨ ∃ v, is_val v ∧ steps e v ∧ steps (K v) e'.
+  Proof.
+    intros HK [n Hstps]%steps_nsteps.
+    revert e e' HK Hstps.
+    induction n; intros e e' HK Hstps.
+    - inversion Hstps; subst; left; eexists _; split; [eauto|apply steps_refl].
+    - inversion Hstps as [|? ? ex]; subst.
+      destruct (step_under_ectx K e ex) as [|(e'' & He''1 & He''2)];
+        [assumption|assumption| |subst].
+      + right; eexists e; split; [assumption|].
+        split; [apply steps_refl|eapply nsteps_steps; eassumption].
+      + destruct (IHn e'' e') as [(? & -> &?)|(?&?&?&?)]; [assumption|assumption| |].
+        * left; eexists; split; [reflexivity|eapply steps_trans; [apply step_steps|]; eauto].
+        * right; eexists _; split; [eassumption|].
+          split; [eapply steps_trans; [apply step_steps|]; eauto|assumption].
+  Qed.
+
   Lemma Safe_bind (P Q : expr → Prop) e K :
     is_ectx K → Safe P e → (∀ v, is_val v → P v → Safe Q (K v)) → Safe Q (K e).
   Proof.
     intros HK He HKSf e' Hstps.
-    remember (K e) as Ke.
-    revert e HeqKe He.
-    pattern Ke; pattern e'.
-    match goal with
-    | |- (λ e2, (λ e1, ?P) _) _ => simpl; apply (steps_ind (λ e1 e2, P))
-    end; [| |assumption]; clear e' Ke Hstps.
-    - intros ? e ? He; subst.
-      destruct (is_val_dec (K e)).
-      + assert (is_val e) by (eapply is_val_under_ectx; eauto).
-        eapply (HKSf e);
-          [assumption|eapply Safe_val_inv; assumption| apply steps_refl].
-      + destruct (is_val_dec e).
-        * eapply (HKSf e);
-          [assumption|eapply Safe_val_inv; assumption| apply steps_refl].
-        * destruct (He e) as [|[e' He']]; [apply steps_refl|tauto|].
-          right; eexists; apply ectx_step; eauto.
-    - intros e e' e'' Hstp Hstps IHstps ei ? Hei; subst.
-      pose proof Hstp as Hvlstp; apply step_under_ectx in Hvlstp as [Hvl|[e3 [He31 He32]]];
-        [|subst|assumption].
-      + eapply (HKSf ei);
-          [assumption|eapply Safe_val_inv; assumption| apply steps_eq_or_step_iff; eauto].
-      + eapply IHstps; [reflexivity|].
-        eapply Safe_step; eauto.
+    apply steps_under_ectx in Hstps as [(e'' & -> & He'')|(v & Hv & Hv1 & Hv2)]; [| |assumption].
+    - apply He in He'' as [[Hie'' HPe'']|[e3 He3]].
+      + eapply HKSf; [eassumption|eassumption|apply steps_refl].
+      + right; eexists; apply ectx_step; eauto.
+    - apply He in Hv1 as [[]|[]]; [|exfalso; eapply val_no_step; eauto; fail].
+      eapply HKSf; [eassumption|assumption|assumption].
   Qed.
 
   Definition Normalizes (P : expr → Prop) (e : expr) := ∃ v, is_val v ∧ steps e v ∧ P v.
@@ -265,6 +306,129 @@ Section language.
     exists w; repeat split; [assumption| |assumption].
     eapply steps_trans; [|eassumption].
     apply ectx_steps; assumption.
+  Qed.
+
+  Lemma val_nsteps_eq n e e' : is_val e → nsteps n e e' → n = 0 ∧ e = e'.
+  Proof.
+    inversion 2; subst; [split; reflexivity|].
+    exfalso; eapply val_no_step; eauto.
+  Qed.
+
+  Lemma nsteps_eq_or_step_iff n e e' :
+    nsteps n e e' ↔ (n = 0 ∧ e = e') ∨ ∃ n' e'', n = S n' ∧ step e e'' ∧ nsteps n' e'' e'.
+  Proof.
+    split.
+    - intros Hsteps.
+      inversion Hsteps; subst.
+      + left; auto.
+      + right; eexists _, _; split; [reflexivity|]; split; [eassumption|eassumption].
+    - intros [[-> ->]|(?&?&->&?&?)]; [constructor|econstructor; eauto].
+  Qed.
+
+  Lemma ectx_nsteps n e e' K : is_ectx K → nsteps n e e' → nsteps n (K e) (K e').
+  Proof. induction 2; econstructor; eauto using ectx_step. Qed.
+
+  Definition SISafe (P : nat → expr → Prop) (n : nat) (e : expr) :=
+    ∀ k e', k ≤ n → nsteps k e e' → (is_val e' ∧ P (n - k) e') ∨ ∃ e'', step e' e''.
+
+  Lemma SISafe_mono (P Q : nat → expr → Prop) n e :
+    (∀ n' v, n' ≤ n → P n' v → Q n' v) → SISafe P n e → SISafe Q n e.
+  Proof.
+    intros HPQ HSf ??? Hstps.
+    apply HSf in Hstps as [?|?]; [|auto; fail|lia].
+    left; split; [tauto|apply HPQ; [lia|tauto]].
+  Qed.
+
+  Lemma SISafe_val (P : nat → expr → Prop) n e : is_val e → P n e → SISafe P n e.
+  Proof.
+    intros He HPe k e' Hk Hstp.
+    left.
+    apply val_nsteps_eq in Hstp as [? ?]; subst; [|assumption].
+    replace (n - 0) with n by lia; auto.
+  Qed.
+
+  Lemma SISafe_val_inv (P : nat → expr → Prop) n e : is_val e → SISafe P n e → P n e.
+  Proof.
+    unfold Safe; intros He HSf.
+    destruct (HSf 0 e) as [[Hiv HP]|[e' He']]; [lia|apply nsteps_refl| |].
+    - replace (n - 0) with n in HP by lia; trivial.
+    - contradict He'; apply val_no_step; trivial.
+  Qed.
+
+  Lemma SISafe_step (P : nat → expr → Prop) e e' n :
+    step e e' → SISafe P (S n) e → SISafe P n e'.
+  Proof.
+    intros Hstep HSf k ei Hk Hsteps.
+    apply (HSf (S k)); [lia|].
+    econstructor; eauto.
+  Qed.
+
+  Lemma SISafe_det_step_back (P : nat → expr → Prop) e e' n :
+    det_step e e' → (0 < n → SISafe P (n - 1) e') → SISafe P n e.
+  Proof.
+    intros Hdstep HSf k ei Hk Hsteps.
+    apply nsteps_eq_or_step_iff in Hsteps as [[-> ->]|(m & e'' & -> & He''1 & He''2)].
+    - right; eexists; apply Hdstep.
+    - apply Hdstep in He''1; subst.
+      destruct n as [|n]; [lia|].
+      pose proof (λ H, HSf H m ei) as HSf'. simpl in *.
+      replace (n - 0) with n in HSf' by lia.
+      apply HSf'; [lia|lia|assumption].
+  Qed.
+
+  Lemma SISafe_head_step_back (P : nat → expr → Prop) e e' n :
+    det_head_step e e' → (0 < n → SISafe P (n - 1) e') → SISafe P n e.
+  Proof.
+    intros.
+    eapply SISafe_det_step_back; [apply det_head_step_det_step|]; eassumption.
+  Qed.
+
+  Lemma nsteps_under_ectx n K e e' :
+    is_ectx K → nsteps n (K e) e' →
+    (∃ e'', e' = K e'' ∧ nsteps n e e'') ∨
+      ∃ k v, k ≤ n ∧ is_val v ∧ nsteps k e v ∧ nsteps (n - k) (K v) e'.
+  Proof.
+    revert e e'.
+    induction n; intros e e' HK Hstps.
+    - inversion Hstps; subst; left; eexists _; split; [eauto|econstructor].
+    - inversion Hstps as [|? ? ex]; subst.
+      destruct (step_under_ectx K e ex) as [|(e'' & He''1 & He''2)];
+        [assumption|assumption| |subst].
+      + right; eexists 0, e; split; [lia|split]; [assumption|].
+        split; [econstructor|].
+        rewrite PeanoNat.Nat.sub_0_r; trivial.
+      + destruct (IHn e'' e') as [(? & -> &?)|(?&?&?&?&?&?)]; [assumption|assumption| |].
+        * left; eexists; split; [reflexivity|econstructor; eauto].
+        * right; eexists (S _), _; repeat split; [|eassumption| |eassumption]; [lia|].
+          econstructor; eauto.
+  Qed.
+
+  Lemma SISafe_bind (P Q : nat → expr → Prop) e K n :
+    is_ectx K →
+    SISafe P n e →
+    (∀ k v, k ≤ n → is_val v → P k v → SISafe Q k (K v)) →
+    SISafe Q n (K e).
+  Proof.
+    intros HK He HKSf k e' Hk Hstps.
+    apply nsteps_under_ectx in Hstps as [(e'' & -> & He'')|(m & ? & v & Hv & Hv1 & Hv2)];
+      [| |assumption].
+    - apply He in He'' as [[Hie'' HPe'']|[e3 He3]]; [| |lia].
+      + apply HKSf in HPe''; [|lia|assumption].
+        pose proof (HPe'' 0) as HPe3.
+        replace (n - k - 0) with (n - k) in HPe3 by lia.
+        apply HPe3; [lia|]; apply nsteps_refl.
+      + right; eexists; apply ectx_step; eauto.
+    - apply He in Hv1 as [[? HPkv]|[]]; [|exfalso; eapply val_no_step; eauto; fail|lia].
+      apply HKSf in HPkv; [|lia|assumption].
+      specialize (HPkv (k - m) e'); simpl in *.
+      replace (n - m - (k - m)) with (n - k) in HPkv by lia.
+      apply HPkv; [lia |assumption].
+  Qed.
+
+  Lemma SISafe_adequacy P e : (∀ n, SISafe (λ _ v, P v) n e) → Safe P e.
+  Proof.
+    intros HSI e' [n Hstps]%steps_nsteps.
+    eapply (HSI n); [|eassumption]; lia.
   Qed.
 
 End language.
