theories/systemF_rec_cbv.v
@@ -1,0 +1,255 @@
+From Coq.Unicode Require Import Utf8.
+From Coq.Lists Require Import List.
+From Autosubst Require Import Autosubst.
+From Coq.Relations Require Import Relations.
+From ShortLogrels Require Import prelude language.
+
+Inductive expr :=
+| Var (v : var)
+| TT
+| Pair (e1 e2 : expr)
+| Fst (e : expr)
+| Snd (e : expr)
+| Lam (e : {bind expr})
+| App (e1 e2 : expr)
+| TLam (e : expr)
+| TApp (e : expr)
+| Fold (e : expr)
+| Unfold (e : expr).
+
+Global Instance Ids_expr : Ids expr. derive. Defined.
+Global Instance Rename_expr : Rename expr. derive. Defined.
+Global Instance Subst_expr : Subst expr. derive. Defined.
+Global Instance SubstLemmas_expr : SubstLemmas expr. derive. Qed.
+
+Inductive is_val : expr → Prop :=
+| IVTT : is_val TT
+| IVPair e1 e2 : is_val e1 → is_val e2 → is_val (Pair e1 e2)
+| IVLam e : is_val (Lam e)
+| IVTLam e : is_val (TLam e)
+| IVFold e : is_val e → is_val (Fold e).
+
+Inductive type :=
+| TUnit
+| TVar (X : var)
+| TProd (τ1 τ2 : type)
+| TFun (τ1 τ2 : type)
+| TForAll (τ : {bind type})
+| TRec (τ : {bind type}).
+
+Global Instance Ids_type : Ids type. derive. Defined.
+Global Instance Rename_type : Rename type. derive. Defined.
+Global Instance Subst_type : Subst type. derive. Defined.
+Global Instance SubstLemmas_type : SubstLemmas type. derive. Qed.
+
+Definition context := environment type.
+
+Inductive typed : context → expr → type → Prop :=
+| TPVar Γ v τ : lookup Γ v = Some τ → typed Γ (Var v) τ
+| TPTT Γ : typed Γ TT TUnit
+| TPPAIR Γ e1 τ1 e2 τ2 : typed Γ e1 τ1 → typed Γ e2 τ2 → typed Γ (Pair e1 e2) (TProd τ1 τ2)
+| TPFst Γ e τ1 τ2 : typed Γ e (TProd τ1 τ2) → typed Γ (Fst e) τ1
+| TPSnd Γ e τ1 τ2 : typed Γ e (TProd τ1 τ2) → typed Γ (Snd e) τ2
+| TPLam Γ e τ1 τ2 : typed (τ1 :: Γ) e τ2 → typed Γ (Lam e) (TFun τ1 τ2)
+| TPApp Γ e1 e2 τ1 τ2 : typed Γ e1 (TFun τ1 τ2) → typed Γ e2 τ1 → typed Γ (App e1 e2) τ2
+| TPTLam Γ e τ : typed (map (rename (+1)) Γ) e τ → typed Γ (TLam e) (TForAll τ)
+| TPTApp Γ e τ τ' : typed Γ e (TForAll τ) → typed Γ (TApp e) τ.[τ'/]
+| TPFold Γ e τ : typed Γ e τ.[TRec τ/] → typed Γ (Fold e) (TRec τ)
+| TPUnfold Γ e τ : typed Γ e (TRec τ) → typed Γ (Unfold e) τ.[TRec τ/].
+
+Inductive head_step : expr → expr → Prop :=
+| SFst e1 e2 : is_val e1 → is_val e2 → head_step (Fst (Pair e1 e2)) e1
+| SSnd e1 e2 : is_val e1 → is_val e2 → head_step (Snd (Pair e1 e2)) e2
+| SApp e1 e2 : is_val e2 → head_step (App (Lam e1) e2) e1.[e2/]
+| STApp e : head_step (TApp (TLam e)) e
+| STUnfold e : is_val e → head_step (Unfold (Fold e)) e.
+
+Inductive is_ectx : (expr → expr) → Prop :=
+| ECTX_id : is_ectx (λ e, e)
+| ECTX_Fst K : is_ectx K → is_ectx (λ e, Fst (K e))
+| ECTX_Snd K : is_ectx K → is_ectx (λ e, Snd (K e))
+| ECTX_Pair1 K e2 : is_ectx K → is_ectx (λ e, Pair (K e) e2)
+| ECTX_Pair2 e1 K : is_val e1 → is_ectx K → is_ectx (λ e, Pair e1 (K e))
+| ECTX_App1 K e2 : is_ectx K → is_ectx (λ e, App (K e) e2)
+| ECTX_App2 e1 K : is_val e1 → is_ectx K → is_ectx (λ e, App e1 (K e))
+| ECTX_TApp K : is_ectx K → is_ectx (λ e, TApp (K e))
+| ECTX_Fold K : is_ectx K → is_ectx (λ e, Fold (K e))
+| ECTX_Unfold K : is_ectx K → is_ectx (λ e, Unfold (K e)).
+
+Local Hint Constructors is_ectx : is_ectx.
+
+Lemma is_ectx_val : ∀ (e : expr) (K : expr → expr), is_ectx K → is_val (K e) → is_val e.
+Proof.
+  intros e K HK; revert e.
+  induction HK; [trivial; fail|inversion 1; subst; auto .. ].
+Qed.
+
+Lemma is_val_dec e : is_val e ∨ ¬ is_val e.
+Proof.
+  induction e; try (right; inversion 1; fail).
+  - left; constructor.
+  - destruct IHe1; destruct IHe2; [left; constructor; auto; fail|right; inversion 1; tauto .. ].
+  - left; constructor.
+  - left; constructor.
+  - destruct IHe; [left; constructor; assumption|right; inversion 1; subst; tauto].
+Qed.
+
+Lemma ectx_head_step K e e' : is_ectx K → head_step (K e) e' → (∀ f : expr, K f = f) ∨ is_val e.
+Proof.
+  intros HK; revert e e'.
+  induction HK.
+  - left; trivial.
+  - inversion HK; inversion 1; subst; right; [econstructor; eauto|eapply is_ectx_val; eauto .. ].
+  - inversion HK; inversion 1; subst; right; [econstructor; eauto|eapply is_ectx_val; eauto .. ].
+  - inversion HK; inversion 1.
+  - inversion HK; inversion 1.
+  - inversion HK; inversion 1; subst; right; constructor.
+  - inversion 1; subst; right; eapply is_ectx_val; eauto.
+  - inversion HK;inversion 1; subst; right; constructor.
+  - inversion HK;inversion 1; subst; right; constructor.
+  - inversion HK;inversion 1; subst; right; [constructor; assumption|eapply is_ectx_val; eauto].
+Qed.
+
+Lemma ectx_inj K e e' : is_ectx K → K e = K e' → e = e'.
+Proof.
+  intros HK; revert e e'.
+  induction HK; intros e e' Hee.
+  - trivial.
+  - intros; assert (K e = K e') by congruence; auto.
+  - intros; assert (K e = K e') by congruence; auto.
+  - intros; assert (K e = K e') by congruence; auto.
+  - intros; assert (K e = K e') by congruence; auto.
+  - intros; assert (K e = K e') by congruence; auto.
+  - intros; assert (K e = K e') by congruence; auto.
+  - intros; assert (K e = K e') by congruence; auto.
+  - intros; assert (K e = K e') by congruence; auto.
+  - intros; assert (K e = K e') by congruence; auto.
+Qed.
+
+Lemma ectx_compose K K' : is_ectx K → is_ectx K' → is_ectx (λ e : expr, K (K' e)).
+Proof.
+  intros HK; revert K'.
+  induction HK; [trivial| intros; econstructor; eauto .. ].
+Qed.
+
+Lemma ectxs_nesting K e K' e' :
+  is_ectx K → is_ectx K' → K e = K' e' → ¬ is_val e → ¬ is_val e' →
+  (∃ K'' : expr → expr, is_ectx K'' ∧ (∀ f : expr, K f = K' (K'' f)))
+  ∨ (∃ K'' : expr → expr, is_ectx K'' ∧ (∀ f : expr, K' f = K (K'' f))).
+Proof.
+  intros HK; revert e e' K'.
+  induction HK as [|?? IHK|?? IHK | K e2 ? IHK|e1 K Hval ? IHK|K e2 ? IHK|e1 K Hval ? IHK|
+                    K HK IHK| K HK IHK|K HK IHK];
+    intros e e' K' HK' Hee Hnve Hnve'.
+  - right; exists K'; auto.
+  - destruct HK'; [left; exists (λ e, Fst (K e)); auto with is_ectx; fail| |congruence ..].
+    destruct (IHK e e' _ HK') as [[K'' [? HK'']]|[K'' [? HK'']]];
+      [congruence|assumption|assumption| left|right];
+      (exists K''; split; [assumption|intros ?; rewrite HK''; trivial]).
+  - destruct HK'; [left; exists (λ e, Snd (K e)); auto with is_ectx; fail|
+                    congruence| |congruence ..].
+    destruct (IHK e e' _ HK') as [[K'' [? HK'']]|[K'' [? HK'']]];
+      [congruence|assumption| assumption|left|right];
+      (exists K''; split; [assumption|intros ?; rewrite HK''; trivial]).
+  - destruct HK' as [| | | |? ? Hval | | | | |];
+      [left; eexists (λ e, Pair (K e) e2); eauto with is_ectx; fail|
+        congruence|congruence | | |congruence .. ].
+    + simplify_eq Hee; intros; subst.
+      destruct (IHK e e' _ HK') as [[K'' [? HK'']]|[K'' [? HK'']]];
+        [congruence|assumption|assumption|left|right];
+        (exists K''; split; [assumption|intros ?; rewrite HK''; trivial]).
+    + simplify_eq Hee; intros; subst.
+      apply is_ectx_val in Hval; tauto.
+  - destruct HK'; [left; eexists (λ e, Pair e1 (K e)); eauto with is_ectx; fail|
+        congruence|congruence | | |congruence .. ].
+    + simplify_eq Hee; intros; subst.
+      apply is_ectx_val in Hval; tauto.
+    + simplify_eq Hee; intros; subst.
+      destruct (IHK e e' _ HK') as [[K'' [? HK'']]|[K'' [? HK'']]];
+        [congruence|assumption|assumption|left|right];
+        (exists K''; split; [assumption|intros ?; rewrite HK''; trivial]).
+  - destruct HK' as [| | | | | |? ? Hval | | |];
+      [left; exists (λ e, App (K e) e2); auto with is_ectx; fail|
+        congruence|congruence| congruence|congruence| | |congruence|congruence|congruence].
+    + simplify_eq Hee; intros; subst.
+      destruct (IHK e e' _ HK') as [[K'' [? HK'']]|[K'' [? HK'']]];
+      [congruence|assumption|assumption| left|right];
+        (exists K''; split; [assumption|intros ?; rewrite HK''; trivial]).
+    + simplify_eq Hee; intros; subst.
+      apply is_ectx_val in Hval; tauto.
+  - destruct HK';
+      [left; exists (λ e, App e1 (K e)); auto with is_ectx; fail|
+        congruence|congruence| congruence|congruence| | |congruence|congruence|congruence].
+    + simplify_eq Hee; intros; subst.
+      apply is_ectx_val in Hval; tauto.
+    + simplify_eq Hee; intros; subst.
+      destruct (IHK e e' _ HK') as [[K'' [? HK'']]|[K'' [? HK'']]];
+      [congruence|assumption|assumption| left|right];
+        (exists K''; split; [assumption|intros ?; rewrite HK''; trivial]).
+  - destruct HK';
+      [left; exists (λ e, TApp (K e)); auto with is_ectx; fail|
+        congruence|congruence| congruence|congruence|congruence|congruence| |congruence|congruence].
+    simplify_eq Hee; intros; subst.
+    destruct (IHK e e' _ HK') as [[K'' [? HK'']]|[K'' [? HK'']]];
+      [congruence|assumption|assumption| left|right];
+        (exists K''; split; [assumption|intros ?; rewrite HK''; trivial]).
+  - destruct HK';
+      [left; exists (λ e, Fold (K e)); auto with is_ectx; fail|
+        congruence|congruence| congruence|congruence|congruence|congruence|congruence| |congruence].
+    simplify_eq Hee; intros; subst.
+    destruct (IHK e e' _ HK') as [[K'' [? HK'']]|[K'' [? HK'']]];
+      [congruence|assumption|assumption| left|right];
+        (exists K''; split; [assumption|intros ?; rewrite HK''; trivial]).
+  - destruct HK';
+      [left; exists (λ e, Unfold (K e)); auto with is_ectx; fail|
+        congruence|congruence| congruence|congruence|congruence|congruence|congruence|congruence|].
+    simplify_eq Hee; intros; subst.
+    destruct (IHK e e' _ HK') as [[K'' [? HK'']]|[K'' [? HK'']]];
+      [congruence|assumption|assumption| left|right];
+        (exists K''; split; [assumption|intros ?; rewrite HK''; trivial]).
+Qed.
+
+Global Instance stlc_valid_language : valid_language is_val is_ectx head_step.
+Proof.
+  split.
+  - inversion 1; inversion 1.
+  - apply is_ectx_val.
+  - constructor.
+  - apply is_val_dec.
+  - apply ectx_head_step.
+  - apply ectx_inj.
+  - apply ectx_compose.
+  - apply ectxs_nesting.
+Qed.
+
+Lemma det_head_step_fst v1 v2 : is_val v1 → is_val v2 → det_head_step (Fst (Pair v1 v2)) v1.
+Proof.
+  intros; split; [constructor; assumption| inversion 1; subst; reflexivity].
+Qed.
+
+Lemma det_head_step_snd v1 v2 : is_val v1 → is_val v2 → det_head_step (Snd (Pair v1 v2)) v2.
+Proof.
+  intros; split; [constructor; assumption| inversion 1; subst; reflexivity].
+Qed.
+
+Lemma det_head_step_app e v : is_val v → det_head_step (App (Lam e) v) e.[v/].
+Proof.
+  intros; split; [econstructor; assumption| inversion 1; subst; reflexivity].
+Qed.
+
+Lemma det_head_step_tapp e : det_head_step (TApp (TLam e)) e.
+Proof.
+  intros; split; [econstructor; assumption| inversion 1; subst; reflexivity].
+Qed.
+
+Lemma det_head_step_unfold e : is_val e → det_head_step (Unfold (Fold e)) e.
+Proof.
+  intros; split; [econstructor; assumption| inversion 1; subst; reflexivity].
+Qed.
+
+Ltac solve_det_head_step :=
+  solve [eapply det_head_step_fst; eassumption|
+          eapply det_head_step_snd; eassumption|
+          eapply det_head_step_app; eassumption|
+          eapply det_head_step_tapp; eassumption|
+          eapply det_head_step_unfold; eassumption].
