theories/systemF_rec_cbv_safety.v
@@ -1,0 +1,594 @@
+From Coq.Unicode Require Import Utf8.
+From Coq.Lists Require Import List.
+From Autosubst Require Import Autosubst.
+From Coq.Relations Require Import Relations.
+From Coq.micromega Require Import Lia.
+From ShortLogrels Require Import prelude language systemF_rec_cbv.
+
+Local Obligation Tactic := idtac.
+
+Record SIPred :=
+{ sipred :> nat → expr → Prop;
+  sipred_over_val : ∀ n e, sipred n e → is_val e;
+  sipred_down_closed : ∀ n n' e, n' ≤ n → sipred n e → sipred n' e }.
+
+Local Hint Resolve sipred_over_val : core.
+
+Definition expr_rel (P : SIPred) := SISafe P.
+
+Lemma expr_rel_down_closed P n n' e : n' ≤ n → expr_rel P n e → expr_rel P n' e.
+Proof.
+  intros ? Hn ??? Hstps.
+  apply Hn in Hstps as [[]|]; [|right; assumption|lia].
+  left; split; [assumption|].
+  eapply sipred_down_closed; [|eassumption]; lia.
+Qed.
+
+Program Definition SIPred_true : SIPred := {| sipred _ e := is_val e |}.
+Next Obligation. trivial. Qed.
+Next Obligation. trivial. Qed.
+
+Definition SIPred_dist (P1 P2 : SIPred) (n : nat) : Prop := ∀ k e, k < n → P1 k e ↔ P2 k e.
+
+Lemma SIPred_dist_0 P1 P2 : SIPred_dist P1 P2 0.
+Proof. intros ???; lia. Qed.
+Lemma SIPred_dist_le P1 P2 n m : n ≤ m → SIPred_dist P1 P2 m → SIPred_dist P1 P2 n.
+Proof. intros ? Hm ? ? ?; eapply Hm; lia. Qed.
+Lemma SIPred_dist_refl P n: SIPred_dist P P n.
+Proof. unfold SIPred_dist; tauto. Qed.
+Lemma SIPred_dist_sym P1 P2 n: SIPred_dist P1 P2 n → SIPred_dist P2 P1 n.
+Proof. unfold SIPred_dist; firstorder. Qed.
+Lemma SIPred_dist_trans P1 P2 P3 n: SIPred_dist P1 P2 n → SIPred_dist P2 P3 n → SIPred_dist P1 P3 n.
+Proof. intros H12 H23; split; intros ?; [apply H23; [|apply H12]|apply H12; [|apply H23]]; auto. Qed.
+
+Definition NonExpansive (Ψ : SIPred → SIPred) : Prop :=
+  ∀ P1 P2 n, SIPred_dist P1 P2 n → SIPred_dist (Ψ P1) (Ψ P2) n.
+
+Definition NonExpansive2 (Ψ : SIPred → SIPred → SIPred) : Prop :=
+  ∀ P11 P12 P21 P22 n,
+    SIPred_dist P11 P12 n → SIPred_dist P21 P22 n → SIPred_dist (Ψ P11 P12) (Ψ P21 P22) n.
+
+Definition Contractive (Ψ : SIPred → SIPred) : Prop :=
+  ∀ P1 P2 n, SIPred_dist P1 P2 n → SIPred_dist (Ψ P1) (Ψ P2) (S n).
+
+Program Definition later (P : SIPred) : SIPred :=
+  {| sipred n e := match n return Prop with 0 => is_val e | S n' => P n' e end |}.
+Next Obligation. simpl; intros ?[]??; [assumption|eapply sipred_over_val; eauto]. Qed.
+Next Obligation.
+  simpl.
+  intros P n n' e Hle ?.
+  destruct n; destruct n'; [assumption|lia| |].
+  - eapply sipred_over_val; eauto.
+  - eapply sipred_down_closed; [|eassumption]; lia.
+Qed.
+
+Lemma later_0 P e : later P 0 e ↔ is_val e.
+Proof. simpl; tauto. Qed.
+Lemma later_S P n e : later P (S n) e ↔ P n e.
+Proof. simpl; tauto. Qed.
+Lemma later_contractive : Contractive later.
+Proof. intros ??? Hltr [] ??; simpl; [tauto|apply Hltr; lia]. Qed.
+
+Opaque later.
+
+Lemma Contractive_NonExpansive Ψ : Contractive Ψ → NonExpansive Ψ.
+Proof. intros Hcn ???????; eapply Hcn; [eassumption|]; lia. Qed.
+
+Fixpoint iter (Ψ : SIPred → SIPred) (n : nat) : SIPred :=
+  match n with | 0 => SIPred_true | S n' => Ψ (iter Ψ n') end.
+
+Lemma iter_dist Ψ (HΨ : Contractive Ψ) n m : n ≤ m → SIPred_dist (iter Ψ m) (iter Ψ n) n.
+Proof.
+  revert n; induction m as [|m IHm]; intros n Hnm.
+  - replace n with 0 by lia. apply SIPred_dist_refl.
+  - destruct n as [|n].
+    + apply SIPred_dist_0.
+    + simpl. apply HΨ.
+      apply IHm; lia.
+Qed.
+
+Program Definition fixpoint (Ψ : SIPred → SIPred) (HΨ : Contractive Ψ) : SIPred :=
+  {| sipred n v := iter Ψ (S n) n v |}.
+Next Obligation. simpl; intros; eapply sipred_over_val; eauto. Qed.
+Next Obligation.
+  simpl.
+  intros Ψ HΨ n; induction n as [|n IHn]; intros n' e Hle Hn.
+  - replace n' with 0 by lia. trivial.
+  - assert (SIPred_dist (Ψ (iter Ψ (S n))) (Ψ (iter Ψ n')) (S n')) as Hhlp.
+    { apply HΨ. apply iter_dist; [assumption|lia]. }
+    apply Hhlp; [lia|].
+    apply (sipred_down_closed _ (S n)); [lia|trivial].
+Qed.
+
+Lemma Ψ_fixpoint (Ψ : SIPred → SIPred) (HΨ : Contractive Ψ) n e :
+  Ψ (fixpoint Ψ HΨ) n e ↔ Ψ (Ψ (iter Ψ n)) n e.
+Proof.
+  eapply (HΨ _ _ n); [|lia].
+  clear e; intros k e' Hlt; simpl.
+  eapply (HΨ _ _ k); [|lia].
+  apply SIPred_dist_sym; apply iter_dist; [assumption|lia].
+Qed.
+
+Lemma fixpoint_dist (Ψ : SIPred → SIPred) (HΨ : Contractive Ψ) n :
+  SIPred_dist (fixpoint Ψ HΨ) (Ψ (fixpoint Ψ HΨ)) n.
+Proof.
+  intros k e Hlt.
+  rewrite Ψ_fixpoint; simpl.
+  eapply (HΨ _ _ k); [|lia].
+  clear n e Hlt.
+  induction k as [|k IHn].
+  - apply SIPred_dist_0.
+  - intros n e Hlt.
+    simpl.
+    eapply (HΨ _ _ k); [|assumption].
+    trivial.
+Qed.
+
+Lemma fixpoint_unfold (Ψ : SIPred → SIPred) (HΨ : Contractive Ψ) n e :
+  fixpoint Ψ HΨ n e ↔ Ψ (fixpoint Ψ HΨ) n e.
+Proof. eapply (fixpoint_dist _ _ (S n)); lia. Qed.
+
+Lemma fixpoint_ne (Ψ Φ : SIPred → SIPred) (HΨ : Contractive Ψ) (HΦ : Contractive Φ) n :
+  (∀ P, SIPred_dist (Ψ P) (Φ P) n) → SIPred_dist (fixpoint Ψ HΨ) (fixpoint Φ HΦ) n.
+Proof.
+  intros HΨΦ.
+  induction n as [|n IHn].
+  - apply SIPred_dist_0.
+  - eapply SIPred_dist_trans; [apply fixpoint_dist|].
+    eapply SIPred_dist_trans; [|apply SIPred_dist_sym; apply fixpoint_dist].
+    eapply SIPred_dist_trans; [apply HΨΦ|].
+    apply (HΦ _ _ n).
+    apply IHn.
+    intros.
+    eapply SIPred_dist_le; [|apply HΨΦ]; lia.
+Qed.
+
+Opaque fixpoint.
+
+Definition SIEnv := environment SIPred.
+
+Definition SIEnv_dist (Δ1 Δ2 : SIEnv) (n : nat) : Prop :=
+  env_rel (λ P1 P2, SIPred_dist P1 P2 n) Δ1 Δ2.
+
+Lemma SIEnv_dist_le Δ1 Δ2 n m : n ≤ m → SIEnv_dist Δ1 Δ2 m → SIEnv_dist Δ1 Δ2 n.
+Proof. intros ?; apply env_rel_impl; intros ? ?; eapply SIPred_dist_le; trivial. Qed.
+Lemma SIEnv_dist_refl Δ n: SIEnv_dist Δ Δ n.
+Proof. apply env_rel_refl; intros; apply SIPred_dist_refl. Qed.
+Lemma SIEnv_dist_sym Δ1 Δ2 n: SIEnv_dist Δ1 Δ2 n → SIEnv_dist Δ2 Δ1 n.
+Proof. apply env_rel_sym; intros; apply SIPred_dist_sym; trivial. Qed.
+Lemma SIEnv_dist_trans Δ1 Δ2 Δ3 n: SIEnv_dist Δ1 Δ2 n → SIEnv_dist Δ2 Δ3 n → SIEnv_dist Δ1 Δ3 n.
+Proof. apply env_rel_trans; intros; eapply SIPred_dist_trans; eauto. Qed.
+
+Definition NonExpansive_env_map (Ψ : SIEnv → SIPred) : Prop :=
+  ∀ Δ1 Δ2 n, SIEnv_dist Δ1 Δ2 n → SIPred_dist (Ψ Δ1) (Ψ Δ2) n.
+
+Record Interp := mkInterp { irp_fun :> SIEnv → SIPred; irp_ne : NonExpansive_env_map irp_fun }.
+
+Program Definition rel_in_env (X : var) : Interp :=
+  mkInterp (λ Δ, match lookup Δ X return SIPred with Some P => P | None => SIPred_true end) _.
+Next Obligation.
+Proof.
+  intros ? Δ1 Δ2 ?????.
+  destruct (lookup Δ1 X) eqn:Heq.
+  - eapply env_rel_lookup1 in Heq as (?& -> & Hdst); [|eassumption].
+    apply Hdst; trivial.
+  - eapply env_rel_lookup1_None in Heq as ->; [|eassumption].
+    tauto.
+Qed.
+
+Program Definition unit_rel : Interp :=
+  mkInterp (λ _, {| sipred n e := e = TT |}) _.
+Next Obligation. simpl; intros; subst; constructor. Qed.
+Next Obligation. trivial. Qed.
+Next Obligation.
+Proof. intros ???????; tauto. Qed.
+
+Program Definition tprod_rel (interp1 interp2 : Interp) : Interp :=
+  mkInterp (λ Δ, {| sipred n e := ∃ e1 e2, e = Pair e1 e2 ∧ interp1 Δ n e1 ∧ interp2 Δ n e2 |}) _.
+Next Obligation. simpl; intros; firstorder; subst; econstructor; eauto. Qed.
+Next Obligation.
+  simpl; intros; firstorder; subst.
+  eexists _, _; split; [reflexivity|]; split; eapply sipred_down_closed; eauto.
+Qed.
+Next Obligation.
+Proof.
+  intros ?????????; simpl.
+  firstorder; subst.
+  - eexists _, _; split; [reflexivity|].
+    split; (eapply irp_ne; [apply SIEnv_dist_sym| |]); eauto.
+  - eexists _, _; split; [reflexivity|].
+    split; eapply irp_ne; eauto.
+Qed.
+
+Program Definition tfun_rel (interp1 interp2 : Interp) : Interp :=
+  mkInterp
+    (λ Δ,
+      {| sipred n v :=
+          is_val v ∧
+            ∀ n' w, n' ≤ n → interp1 Δ n' w → expr_rel (interp2 Δ) n' (App v w)
+      |}) _.
+Next Obligation. simpl; intros; tauto. Qed.
+Next Obligation.
+  simpl.
+  intros ? ? Δ n n' v Hn'n [? Hv].
+  split; [assumption|].
+  intros k w Hkn' Hw.
+  eapply SISafe_mono; [|eapply Hv; [|eauto]]; [|lia].
+  simpl; intros.
+  eapply sipred_down_closed; [|eassumption]; lia.
+Qed.
+Next Obligation.
+Proof.
+  intros ?????????; simpl.
+  intuition.
+  - eapply SISafe_mono; [|match goal with H : _ |- _ => eapply H end];
+    [|eassumption|eapply irp_ne; [eassumption| |eassumption]]; [|lia].
+    simpl; intros ????.
+    eapply irp_ne; [apply SIEnv_dist_sym; eassumption| |eassumption].
+    lia.
+  - eapply SISafe_mono; [|match goal with H : _ |- _ => apply H end];
+    [|eassumption|eapply irp_ne; [apply SIEnv_dist_sym; eassumption| |eassumption]];
+      [|lia].
+    simpl; intros ????.
+    eapply irp_ne; [eassumption| |eassumption]. lia.
+Qed.
+
+Program Definition tforall_rel (interp : Interp) : Interp :=
+  mkInterp
+    (λ Δ,
+      {| sipred n v :=
+          is_val v ∧
+            ∀ (P : SIPred), SISafe (interp (P :: Δ)) n (TApp v) |})
+    _.
+Next Obligation. simpl; intros; tauto. Qed.
+Next Obligation.
+  simpl; intros interp Δ n n' v Hn'n [? Hv].
+  split; [assumption|].
+  intros P.
+  eapply expr_rel_down_closed; [|eapply Hv]; lia.
+Qed.
+Next Obligation.
+Proof.
+  intros ????????; simpl.
+  intuition.
+  - eapply SISafe_mono; [|match goal with H : _ |- _ => apply H end].
+    simpl; intros ????.
+    eapply irp_ne; [| |eassumption].
+    + apply env_rel_cons; [|apply SIEnv_dist_sym; eassumption].
+      apply SIPred_dist_refl.
+    + lia.
+  - eapply SISafe_mono; [|match goal with H : _ |- _ => apply H end].
+    simpl; intros ????.
+    eapply irp_ne; [| |eassumption].
+    + apply env_rel_cons; [|eassumption].
+      apply SIPred_dist_refl.
+    + lia.
+Qed.
+
+Program Definition trec_rel1 (Ψ : SIPred → SIPred) (P : SIPred) : SIPred :=
+  {| sipred n v := ∃ w, v = Fold w ∧ later (Ψ P) n w |}.
+Next Obligation.
+Proof.
+  simpl; intros ? ? n ? (?& -> &?).
+  destruct n; [constructor; assumption|].
+  constructor; eapply sipred_over_val; eauto.
+Qed.
+Next Obligation.
+Proof.
+  simpl; intros ? P n n' e Hn'n Hv.
+  destruct Hv as (?& -> &?).
+  eexists _; split; [reflexivity|].
+  eapply sipred_down_closed; eauto.
+Qed.
+
+Lemma trec_rel1_ne (Ψ Φ : SIPred → SIPred) P n e :
+  (∀ Q, SIPred_dist (Ψ Q) (Φ Q) n) → trec_rel1 Ψ P n e ↔ trec_rel1 Φ P n e.
+Proof.
+  intros HΨΦ.
+  unfold trec_rel1; simpl.
+  firstorder; subst; (eexists _; split; [reflexivity|]).
+  - eapply (later_contractive _ _ n); [|lia|eassumption].
+    intros ???; symmetry; eapply HΨΦ; eauto.
+  - eapply (later_contractive _ _ n); [|lia|eassumption].
+    intros ???; eapply HΨΦ; eauto.
+Qed.
+
+Lemma trec_rel1_contractive Ψ : NonExpansive Ψ → Contractive (trec_rel1 Ψ).
+Proof.
+  unfold trec_rel1; intros HΨ ??? HPs ???; simpl.
+  eapply HΨ in HPs.
+  apply later_contractive in HPs.
+  firstorder; subst; (eexists _; split; [reflexivity|apply HPs]).
+Qed.
+
+Program Definition trec_rel (interp : Interp) : Interp :=
+  mkInterp (λ Δ, fixpoint (trec_rel1 (λ P, interp (P :: Δ))) _) _.
+Next Obligation.
+Proof.
+  intros ??????.
+  apply trec_rel1_contractive; [|assumption].
+  intros ????.
+  apply irp_ne.
+  apply env_rel_cons; [assumption|].
+  apply SIEnv_dist_refl.
+Qed.
+Next Obligation.
+Proof.
+  intros ????????.
+  eapply fixpoint_ne; [|eassumption].
+  intros P ?.
+  eapply SIPred_dist_trans.
+  { intros z ??.
+    apply trec_rel1_ne.
+    intros ????.
+    eapply irp_ne; [|eassumption].
+    apply env_rel_cons; [apply SIPred_dist_refl|].
+    eapply SIEnv_dist_le; [|eassumption]; lia. }
+  apply SIPred_dist_refl.
+Qed.
+
+Fixpoint val_rel (τ : type) {struct τ} : Interp :=
+  match τ with
+  | TUnit => unit_rel
+  | TVar X => rel_in_env X
+  | TProd τ1 τ2 => tprod_rel (val_rel τ1) (val_rel τ2)
+  | TFun τ1 τ2 => tfun_rel (val_rel τ1) (val_rel τ2)
+  | TForAll τ => tforall_rel (val_rel τ)
+  | TRec τ => trec_rel (val_rel τ)
+  end.
+
+Local Notation env_rel Δ n Γ env := (env_rel (λ τ, val_rel τ Δ n) Γ env).
+
+Lemma val_rel_is_val Δ τ n v : val_rel τ Δ n v → is_val v.
+Proof. apply sipred_over_val. Qed.
+
+Lemma val_rel_weaken_gen Δ1 Δ' Δ2 n τ v :
+  val_rel τ (Δ1 ++ Δ2) n v ↔ val_rel (weaken (length Δ1) (length Δ') τ) (Δ1 ++ Δ' ++ Δ2) n v.
+Proof.
+  revert Δ1 Δ' Δ2 n v.
+  induction τ as [| X | | | |]; intros Δ1 Δ' Δ2 n v.
+  - simpl; tauto.
+  - simpl.
+    rewrite (@weaken_var type); [|apply _]; simpl.
+    unfold rel_in_env.
+    destruct Nat.ltb eqn:Hlt.
+    + apply PeanoNat.Nat.ltb_lt in Hlt.
+      repeat (rewrite lookup_app_l; [|assumption]).
+      tauto.
+    + apply PeanoNat.Nat.ltb_ge in Hlt.
+      rewrite app_assoc.
+      rewrite lookup_app_r; [|assumption].
+      rewrite lookup_app_r; [|rewrite app_length; lia].
+      rewrite app_length.
+      replace (X + length Δ' - (length Δ1 + length Δ')) with (X - length Δ1) by lia.
+      tauto.
+  - split; intros (?&?&?&?&?); eexists _, _; repeat split; eauto;
+      match goal with H : _ |- _ => apply H; eauto | H : _ |- _ => apply <- H; eauto end.
+  - simpl.
+    split; intros [? Happ];
+      split; [assumption|intros; eapply SISafe_mono; [intros|eapply Happ]|
+               assumption|intros; eapply SISafe_mono; [intros|eapply Happ]]; eauto;
+      repeat match goal with H : _ |- _ => apply H; eauto | H : _ |- _ => apply <- H; eauto end.
+  - split; intros [? Htapp].
+    + split; [assumption|].
+      intros ?. eapply SISafe_mono; [|eapply Htapp; fail].
+      intros ???.
+      apply (IHτ (_ :: _)); eassumption.
+    + split; [assumption|].
+      intros ?.
+      eapply SISafe_mono; [|eapply Htapp; fail].
+      intros ?? w Hw.
+      eapply (IHτ (_ :: _)) in Hw; eauto.
+  - simpl.
+    eapply (fixpoint_ne _ _ _ _ (S n)); [|lia].
+    intros P k e Hk.
+    split; intros [? [? Hltr]]; subst; eexists _; (split; [reflexivity|]).
+    + destruct k; [rewrite later_0; rewrite later_0 in Hltr; assumption|].
+      rewrite later_S; rewrite later_S in Hltr.
+      apply (IHτ (_ :: _)); trivial.
+    + destruct k; [rewrite later_0; rewrite later_0 in Hltr; assumption|].
+      rewrite later_S; rewrite later_S in Hltr.
+      apply (IHτ (_ :: _)) in Hltr; trivial.
+Qed.
+
+Lemma val_rel_weaken Δ1 Δ2 τ n v : val_rel τ Δ2 n v ↔ val_rel τ.[ren (+length Δ1)] (Δ1 ++ Δ2) n v.
+Proof.
+  rewrite (val_rel_weaken_gen nil Δ1 Δ2); simpl.
+  rewrite weaken_0; asimpl; tauto.
+Qed.
+
+Lemma env_rel_weaken Δ1 Δ' Δ2 n Γ env :
+  env_rel (Δ1 ++ Δ2) n Γ env ↔
+  env_rel (Δ1 ++ Δ' ++ Δ2) n (map (weaken (length Δ1) (length Δ')) Γ) env.
+Proof.
+  revert env.
+  induction Γ as [|τ Γ IHΓ]; intros env.
+  - split.
+    + intros ->%env_rel_inv_nil_l; apply env_rel_nil.
+    + intros ->%env_rel_inv_nil_l; apply env_rel_nil.
+  - split; simpl.
+    + intros (?&?&->&?&?)%env_rel_inv_cons_l.
+      apply env_rel_cons; [|apply IHΓ; eauto; fail].
+      apply val_rel_weaken_gen; auto.
+    + intros (?&?&->&?&?)%env_rel_inv_cons_l.
+      apply env_rel_cons; [|apply IHΓ; eauto; fail].
+      apply <- val_rel_weaken_gen; eauto.
+Qed.
+
+Lemma env_rel_weaken1 P Δ Γ n env :
+  env_rel Δ n Γ env → env_rel (P :: Δ) n (map (rename (+1)) Γ) env.
+Proof. rewrite (env_rel_weaken (nil) (cons P nil) Δ); simpl; rewrite weaken_0; trivial. Qed.
+
+Lemma val_rel_subst_gen Δ1 τ' Δ2 τ n v :
+  val_rel τ (Δ1 ++ (val_rel τ' Δ2) :: Δ2) n v ↔
+  val_rel τ.[upn (length Δ1) (τ'.: ids)] (Δ1 ++ Δ2) n v.
+Proof.
+  revert Δ1 Δ2 n v.
+  induction τ as [| X | | | |]; intros Δ1 Δ2 n v.
+  - simpl; tauto.
+  - asimpl.
+    rewrite upn_ext.
+    destruct Nat.ltb eqn:Hlt.
+    + apply PeanoNat.Nat.ltb_lt in Hlt.
+      simpl; unfold rel_in_env; simpl.
+      repeat (rewrite lookup_app_l; [|assumption]); tauto.
+    + apply PeanoNat.Nat.ltb_ge in Hlt.
+      destruct (PeanoNat.Nat.eq_dec X (length Δ1)) as [->|].
+      * rewrite PeanoNat.Nat.sub_diag; asimpl.
+        unfold rel_in_env.
+        rewrite lookup_app_r; [|lia].
+        rewrite PeanoNat.Nat.sub_diag; simpl.
+        rewrite <- val_rel_weaken; intuition; eauto using val_rel_is_val.
+      * simpl; unfold rel_in_env; simpl.
+        rewrite lookup_app_r; [|lia].
+        destruct (X - length Δ1) as [|z] eqn:Heq; [lia|].
+        simpl; unfold rel_in_env; simpl.
+        rewrite lookup_app_r; [|lia].
+        replace (length Δ1 + z - length Δ1) with z by lia.
+        tauto.
+  - split; intros (?&?&?&?&?); eexists _, _; repeat split; eauto;
+      match goal with H : _ |- _ => apply H; eauto | H : _ |- _ => apply <- H; eauto end.
+  - simpl.
+    split; intros [? Happ];
+      split; [assumption|intros; eapply SISafe_mono; [intros|eapply Happ]|
+               assumption|intros; eapply SISafe_mono; [intros|eapply Happ]]; eauto;
+      repeat match goal with H : _ |- _ => apply H; eauto | H : _ |- _ => apply <- H; eauto end.
+  - split; intros [? Htapp].
+    + split; [assumption|].
+      intros ?. eapply SISafe_mono; [|eapply Htapp; fail].
+      intros ???.
+      apply (IHτ (_ :: _)); eassumption.
+    + split; [assumption|].
+      intros ?.
+      eapply SISafe_mono; [|eapply Htapp; fail].
+      intros ?? w Hw.
+      eapply (IHτ (_ :: _)) in Hw; eauto.
+  - simpl.
+    eapply (fixpoint_ne _ _ _ _ (S n)); [|lia].
+    intros P k e Hk.
+    split; intros [? [? Hltr]]; subst; eexists _; (split; [reflexivity|]).
+    + destruct k; [rewrite later_0; rewrite later_0 in Hltr; assumption|].
+      rewrite later_S; rewrite later_S in Hltr.
+      apply (IHτ (_ :: _)); trivial.
+    + destruct k; [rewrite later_0; rewrite later_0 in Hltr; assumption|].
+      rewrite later_S; rewrite later_S in Hltr.
+      apply (IHτ (_ :: _)) in Hltr; trivial.
+Qed.
+
+Lemma val_rel_subst τ' Δ τ n v : val_rel τ (val_rel τ' Δ :: Δ) n v ↔ val_rel τ.[τ'/] Δ n v.
+Proof. apply (val_rel_subst_gen nil). Qed.
+
+Lemma env_rel_down_closed Δ n n' Γ env : n' ≤ n → env_rel Δ n Γ env → env_rel Δ n' Γ env.
+Proof.
+  revert env.
+  induction Γ as [|τ Γ IHΓ]; intros env ?.
+  - intros ->%env_rel_inv_nil_l; apply env_rel_nil.
+  - simpl.
+    intros (?&?&->&?&?)%env_rel_inv_cons_l.
+    apply env_rel_cons; [|apply IHΓ; eauto; fail].
+    eapply sipred_down_closed; eauto.
+Qed.
+
+Theorem Fundamental Γ e τ :
+  typed Γ e τ → ∀ n Δ env, env_rel Δ n Γ env → expr_rel (val_rel τ Δ) n e.[env_subst env].
+Proof.
+  intros Htp.
+  induction Htp; intros n Δ env Henv; simpl.
+  - simpl.
+    assert (val_rel τ Δ n (env_subst env v)).
+    { eapply env_rel_lookup1 in Henv as [? [? ?]]; [|eauto; fail].
+      erewrite env_subst_lookup; eauto. }
+    apply SISafe_val; [eapply val_rel_is_val; eauto|].
+    eapply sipred_down_closed; [|eassumption]; lia.
+  - apply SISafe_val; [constructor|simpl; trivial].
+  - eapply (SISafe_bind _ _ _ (λ e, Pair e _));
+      [repeat econstructor; fail|eapply IHHtp1; eauto; fail|].
+    intros k v1 ? Hv11 Hv12; simpl.
+    eapply (SISafe_bind _ _ _ (λ e, Pair _ e)).
+    { repeat econstructor; trivial. }
+    { eapply IHHtp2; eapply env_rel_down_closed; [|eassumption]; trivial. }
+    intros k' ? v2 Hv21 Hv22.
+    apply SISafe_val; [constructor; trivial; fail|].
+    eexists _, _; split; [reflexivity|].
+    split; [|assumption].
+    eapply sipred_down_closed; [|eassumption]; assumption.
+  - eapply (SISafe_bind _ _ _ (λ e, Fst e));
+      [repeat econstructor; fail|apply IHHtp; eassumption; fail|].
+    intros ? v ? Hv1 (v1 & v2 & -> & Hv1r & Hv2r).
+    inversion Hv1; subst.
+    eapply SISafe_head_step_back; [solve_det_head_step|intros ?].
+    apply SISafe_val; [assumption|].
+    eapply sipred_down_closed; [|eassumption]; lia.
+  - eapply (SISafe_bind _ _ _ (λ e, Snd e));
+      [repeat econstructor; fail|apply IHHtp; eassumption; fail|].
+    intros ? v ? Hv1 (v1 & v2 & -> & Hv1r & Hv2r).
+    inversion Hv1; subst.
+    eapply SISafe_head_step_back; [solve_det_head_step|intros ?].
+    apply SISafe_val; [assumption|].
+    eapply sipred_down_closed; [|eassumption]; lia.
+  - apply SISafe_val; [constructor; fail|].
+    simpl.
+    split; [constructor; fail|].
+    intros ? w ? Hw.
+    assert (is_val w) by (eapply val_rel_is_val; eauto).
+    eapply SISafe_head_step_back; [solve_det_head_step|intros ?].
+    asimpl.
+    apply (IHHtp _ Δ (_ :: _)).
+    apply env_rel_cons;
+      [eapply sipred_down_closed; [|eassumption]|eapply env_rel_down_closed; [|eassumption]]; lia.
+  - eapply (SISafe_bind _ _ _ (λ e, App e _));
+      [repeat econstructor; fail|apply IHHtp1; eassumption; fail|].
+    intros ? v1 ? Hv11 Hv12.
+    eapply (SISafe_bind _ _ _ (λ e, App _ e)); [| |].
+    { repeat econstructor; trivial. }
+    { eapply IHHtp2; eapply env_rel_down_closed; [|eassumption]; trivial. }
+    intros ? v2 ? Hv21 Hv22.
+    apply Hv12; trivial.
+  - apply SISafe_val; [constructor; fail|].
+    split; [constructor; fail|].
+    intros P.
+    eapply SISafe_head_step_back; [solve_det_head_step|intros ?].
+    apply IHHtp.
+    apply env_rel_weaken1; trivial.
+    eapply env_rel_down_closed; [|eassumption]; lia.
+  - eapply (SISafe_bind _ _ _ (λ e, TApp e));
+      [repeat econstructor; fail|apply IHHtp; eassumption; fail|].
+    intros ? v ? ? [? Hv].
+    eapply SISafe_mono; [|apply Hv; fail].
+    intros ????; rewrite <- val_rel_subst; eassumption.
+  - eapply SISafe_mono.
+    { intros ??? HP. rewrite fixpoint_unfold; exact HP. }
+    eapply (SISafe_bind _ _ _ (λ e, Fold e));
+      [repeat econstructor; fail|apply IHHtp; eassumption; fail|].
+    intros ? v ? ? Hv.
+    apply SISafe_val; [econstructor; assumption|].
+    eexists _; split; [reflexivity|].
+    destruct k; [apply later_0; assumption|].
+    apply later_S.
+    apply (val_rel_subst (TRec _)).
+    eapply sipred_down_closed; [|eassumption]; lia.
+  - eapply (SISafe_bind _ _ _ (λ e, Unfold e));
+      [repeat econstructor; fail|apply IHHtp; eassumption; fail|].
+    intros ? v ? Hiv Hv.
+    simpl in *.
+    rewrite fixpoint_unfold in Hv.
+    destruct Hv as (w&->&Hw).
+    inversion Hiv; subst.
+    eapply SISafe_head_step_back; [solve_det_head_step|intros ?].
+    apply SISafe_val; [assumption|].
+    destruct k; [lia|].
+    rewrite later_S in Hw.
+    apply (val_rel_subst (TRec _)).
+    simpl.
+    replace (k - 0) with k by lia.
+    assumption.
+Qed.
+
+Corollary type_safety e τ : typed nil e τ → Safe (λ _, True) e.
+Proof.
+  intros Htp.
+  apply SISafe_adequacy; intros n.
+  eapply SISafe_mono; [tauto|].
+  replace e with e.[env_subst nil] by (asimpl; reflexivity).
+  eapply (Fundamental nil _ _ Htp _ nil); apply env_rel_nil.
+Qed.
